Modify function

TCR/Data/SegmentTree/Basic.lean
@@ -6,17 +6,21 @@ Authors: Markus Himmel
 module
 
 import TCR.Data.Vector
+import TCR.Data.Nat
 
 namespace TCR
 
 /-- A vector of size `2 * n` is an `op`-segment tree if, when interpreted as a binary tree,
 it satisfies the heap-like property that the parent is always the `op` of the children. -/
 structure IsSegmentTree (op : α → α → α) (neutral : α) (v : Vector α (2 * n)) : Prop where
+  /-- The unused zero-th element of `v` is the neutral element, to ensure that segment trees on
+  a given underlying array are unique. -/
   zero_eq : ∀ (h : 0 < 2 * n), v[0] = neutral
   /-- Given `0 < i < n`, `v[i] = op v[2 * i + 1] v[2 * i + 2]`. -/
-  op_eq : ∀ (i : Nat) (_ : 0 < i) (hi : i < n), v[i] = op v[2 * i] (v[(2 * i + 1)]?.getD neutral)
+  op_eq : ∀ (i : Nat) (_ : 0 < i) (hi : i < n), v[i] = op v[2 * i] v[2 * i + 1]
 
 /-- Creates a new `op`-segment tree on the vector `v`. -/
+@[inline]
 def mkSegmentTree (op : α → α → α) (neutral : α) (v : Vector α n) : Vector α (2 * n) :=
   if h : n = 0 then
     Vector.mk #[] (by simp [h])
@@ -24,10 +28,10 @@ def mkSegmentTree (op : α → α → α) (neutral : α) (v : Vector α n) : Vec
     let vec := Vector.mk (Array.replicate n neutral ++ v.toArray) (by grind)
     loop vec (n - 1) (by omega)
 where
-  loop (vec : Vector α (2 * n)) (idx : Nat) (hidx : idx < n) : Vector α (2 * n) :=
+  @[specialize] loop (vec : Vector α (2 * n)) (idx : Nat) (hidx : idx < n) : Vector α (2 * n) :=
     match h : idx with
     | 0 => vec
-    | idx' + 1 => loop (vec.set (idx' + 1) (op vec[2 * (idx' + 1)] (vec.getD (2 * (idx' + 1) + 1) neutral))) idx' (by grind)
+    | idx' + 1 => loop (vec.set (idx' + 1) (op vec[2 * (idx' + 1)] vec[2 * (idx' + 1) + 1])) idx' (by grind)
 
 theorem isSegmentTree_mkSegmentTree {op : α → α → α} {neutral : α} {v : Vector α n} :
     IsSegmentTree op neutral (mkSegmentTree op neutral v) := by
@@ -40,8 +44,8 @@ where
   loop {vec : Vector α (2 * n)} (idx : Nat) (hidx : idx < n)
       (h₀ : vec[0] = neutral)
       (h : ∀ idx', 0 < idx' → idx < idx' → (h : idx' < n) →
-        vec[idx'] = op vec[2 * idx'] (vec.getD (2 * idx' + 1) neutral)) :
-      IsSegmentTree op neutral (mkSegmentTree.loop op neutral vec idx hidx) := by
+        vec[idx'] = op vec[2 * idx'] vec[2 * idx' + 1]) :
+      IsSegmentTree op neutral (mkSegmentTree.loop op vec idx hidx) := by
     fun_induction mkSegmentTree.loop with
     | case1 => exact ⟨by simp_all, by simpa using h⟩
     | case2 vec idx' hidx ih =>
@@ -51,8 +55,8 @@ where
         split
         · rename_i h
           subst h
-          rw [Vector.getElem_set_ne _ _ (by omega), Vector.getD_set_ne (by omega)]
-        · rw [Vector.getElem_set_ne _ _ (by omega), Vector.getD_set_ne (by omega)]
+          rw [Vector.getElem_set_ne _ _ (by omega), Vector.getElem_set_ne _ _ (by omega)]
+        · rw [Vector.getElem_set_ne _ _ (by omega), Vector.getElem_set_ne _ _ (by omega)]
           apply h <;> omega
 
 /-- Given a segment tree, extracts the underlying data by copying it. -/
@@ -76,7 +80,7 @@ theorem underlying_mkSegmentTree {op : α → α → α} {neutral : α} {v : Vec
   split
   · simp_all [underlying]
   suffices ∀ (vec : Vector α (2 * n)) idx hidx,
-      (mkSegmentTree.loop op neutral vec idx hidx).extract n (2 * n) = vec.extract n (2 * n) by
+      (mkSegmentTree.loop op vec idx hidx).extract n (2 * n) = vec.extract n (2 * n) by
     simp [underlying, this]
     grind
   intro vec idx hidx
@@ -99,6 +103,60 @@ theorem IsSegmentTree.underlying_inj (v v' : Vector α (2 * n))
     have := ih (2 * i - n)
     grind (splits := 12) [getElem_eq_getElem_underlying]
 
+/-- Modifies the underlying array of the segment tree at position `i` using `f` and restores the segment tree
+property. -/
+@[inline]
+def modify (op : α → α → α) (v : Vector α (2 * n)) (i : Nat) (hi : i < n) (f : α → α) : Vector α (2 * n) :=
+  loop (v.modify (n + i) f) (n + i) (by omega) (by omega)
+where
+  @[specialize] loop (vec : Vector α (2 * n)) (idx : Nat) (hidx₀ : idx ≠ 0) (hidx : idx < 2 * n) : Vector α (2 * n) :=
+    if h : idx = 1 then
+      vec
+    else
+      loop (vec.set (idx / 2) (op vec[idx] (vec[idx ^^^ 1]'(by grind [Nat.xor_one_eq])))) (idx / 2) (by omega) (by omega)
 
+@[simp]
+theorem underlying_modify {op : α → α → α} {v : Vector α (2 * n)} {i : Nat} {hi : i < n} {f : α → α} :
+    underlying (modify op v i hi f) = (underlying v).modify i f := by
+  suffices ∀ (vec : Vector α (2 * n)) idx hidx₀ hidx, underlying (modify.loop op i hi f vec idx hidx₀ hidx) = underlying vec by
+    simp only [modify, this]
+    simp only [underlying, Vector.modify_cast, Vector.cast_eq_cast, Vector.cast_rfl]
+    ext j hj
+    simp [Vector.getElem_modify]
+  intro vec idx hidx₀ hidx
+  fun_induction modify.loop with
+  | case1 => rfl
+  | case2 vec idx hidx₀ hidx hidx' ih =>
+    rw [ih, underlying, underlying, Vector.cast_eq_cast, Vector.cast_rfl,
+      Vector.extract_set, dif_pos (by grind)]
+
+theorem IsSegmentTree.modify {op : α → α → α} [Std.Commutative op] {neutral : α} {v : Vector α (2 * n)} (hv : IsSegmentTree op neutral v)
+    {i : Nat} (hi : i < n) (f : α → α) : IsSegmentTree op neutral (modify op v i hi f) := by
+  rw [TCR.modify]
+  apply loop <;> grind [Vector.getElem_modify_of_ne, IsSegmentTree.zero_eq, IsSegmentTree.op_eq]
+where
+  loop {vec : Vector α (2 * n)} {idx hidx₀ hidx} (h₀ : vec[0] = neutral)
+      (h : ∀ (i : Nat) (_ : 0 < i) (hi : i < n) (_ : i ≠ idx / 2), vec[i] = op vec[2 * i] vec[2 * i + 1]) :
+      IsSegmentTree op neutral (modify.loop op i hi f vec idx hidx₀ hidx) := by
+    fun_induction modify.loop with
+    | case1 vec h₁ h₂ => exact ⟨by simp [h₀], fun j hj hj' => h _ hj hj' (by omega)⟩
+    | case2 vec idx hidx₀ hidx h' ih =>
+      apply ih
+      · rw [Vector.getElem_set_ne _ _ (by omega), h₀]
+      · intro j hj hj' hj''
+        conv => rhs; rw [Vector.getElem_set_ne _ _ (by omega), Vector.getElem_set_ne _ _ (by omega)]
+        rw [Vector.getElem_set]
+        split <;> rename_i hj₀
+        · subst hj₀
+          simp only [Nat.xor_one_eq]
+          have := Nat.div_add_mod n 2
+          split <;> rename_i hidx2
+          · have : idx = 2 * (idx / 2) := by grind
+            grind
+          · have : idx = 2 * (idx / 2) + 1 := by grind
+            rw [Std.Commutative.comm (op := op)]
+            congr
+            grind
+        · exact h _ hj hj' (by omega)
 
 end TCR
