TCR/Data/Nat.lean
@@ -1,0 +1,29 @@
+/-
+Copyright (c) 2025 Markus Himmel. All rights reserved.
+Released under Apache 2.0 license as described in the file LICENSE.
+Authors: Markus Himmel
+-/
+module
+
+public theorem Nat.two_mul_add_eq_or_of_lt {b : Nat} (hb : b < 2) (a : Nat) : 2 * a + b = 2 * a ||| b := by
+  simpa using Nat.two_pow_add_eq_or_of_lt (i := 1) (by simpa using hb) a
+
+@[simp]
+public theorem Nat.testBit_two_mul : (2 * a).testBit j = (decide (j ≥ 1) && a.testBit (j - 1)) := by
+  simpa using Nat.testBit_two_pow_mul (i := 1)
+
+@[simp]
+public theorem Nat.testBit_mul_two : (a * 2).testBit j = (decide (j ≥ 1) && a.testBit (j - 1)) := by
+  simpa using Nat.testBit_mul_two_pow (i := 1) ..
+
+public theorem Nat.xor_one_eq {n : Nat} : n ^^^ 1 = if n % 2 = 0 then n + 1 else n - 1 := by
+  split <;> rename_i h
+  · rw [← Nat.div_add_mod n 2, h, Nat.add_zero, Nat.two_mul_add_eq_or_of_lt (by omega)]
+    apply Nat.eq_of_testBit_eq
+    simp; grind
+  · rw [← Nat.div_add_mod n 2, Nat.mod_two_not_eq_zero.1 h, Nat.add_one_sub_one]
+    apply Nat.eq_of_testBit_eq
+    simp; grind
+
+public theorem Nat.xor_one_le {n : Nat} : n ^^^ 1 ≤ n + 1 := by
+  grind [Nat.xor_one_eq]
